Makefile
@@ -1,89 +1,13 @@
-.PHONY: verify clean
+INCLUDE_PATHS=parsers
+include Makefile.common
 
-FSTAR_HOME ?= everest/FStar
-QD_HOME ?= everest/quackyducky
-LOWPARSE_HOME ?= $(QD_HOME)/src/lowparse
-KREMLIN_HOME ?= everest/kremlin
-
-# List the files that should be verified by verify-extra and verify-all
-EXTRA=
-
-# List the files that should NOT be verified at all
-FLAKY=
-
-# List the files that should be verified by verify-core and verify-all
-# Those files are the roots from where all dependencies are computed
-FSTAR_FILES := Veritas.BinTree.fsti Veritas.BinTree.fst \
-               Veritas.Key.fsti Veritas.Record.fsti \
-               Veritas.SeqAux.fsti Veritas.SeqAux.fst \
-               Veritas.SeqMachine.fsti Veritas.SeqMachine.fst \
-               Veritas.State.fsti \
-               Veritas.StateSeqMachine.fsti Veritas.StateSeqMachine.fst \
-               Veritas.MultiSet.fsti Veritas.MultiSet.fst \
-               Veritas.MultiSetHash.fsti \
-               Veritas.Hash.fsti \
-               Veritas.Interleave.fsti Veritas.Interleave.fst \
-               Veritas.Verifier.fst \
-	       Veritas.Verifier.Thread.fsti Veritas.Verifier.Thread.fst \
-               Veritas.Verifier.Global.fsti Veritas.Verifier.Global.fst \
-               Veritas.EAC.fsti Veritas.EAC.fst \
-               Veritas.Verifier.TSLog.fsti Veritas.Verifier.TSLog.fst \
-	       Veritas.Verifier.Blum.fsti Veritas.Verifier.Blum.fst \
-               Veritas.Verifier.Merkle.fsti Veritas.Verifier.Merkle.fst \
-               Veritas.Verifier.EAC.fst \
-               Veritas.Verifier.Correctness.fst
-
-
-# Uncomment the definition of PROFILE below, if you want some basic
-# profiling of F* runs on Veritas files It will report the time spent
-# on typechecking your file And the time spent in SMT, which is
-# included in the total typechecking time
-
-# PROFILE=--profile Veritas --profile_component 'FStar.Universal.tc_source_file FStar.SMTEncoding'
-
-OTHERFLAGS+=$(PROFILE)
-
-# 271: theory symbols in smt patters
-WARN_ERROR=--warn_error -271
-SMT_OPTIONS=--z3cliopt 'timeout=600000' --z3cliopt 'smt.arith.nl=false' \
-	    --smtencoding.elim_box true \
-	    --smtencoding.l_arith_repr native \
-	    --smtencoding.nl_arith_repr wrapped
-OTHERFLAGS+=$(WARN_ERROR) $(SMT_OPTIONS)
-ALREADY_CACHED=--already_cached 'Prims FStar LowStar'
-
-FSTAR=fstar.exe $(OTHERFLAGS) $(ALREADY_CACHED) --cache_dir cache
-
-# A place to put all the emitted .ml files
-OUTPUT_DIRECTORY ?= _output
-
-INCLUDE_PATHS=parsers $(OUTPUT_DIRECTORY) $(LOWPARSE_HOME) $(KREMLIN_HOME)/kremlib
-
-FSTAR_OPTIONS=--odir $(OUTPUT_DIRECTORY) \
-	      --cache_dir $(OUTPUT_DIRECTORY) \
-	      $(addprefix --include , $(INCLUDE_PATHS))
-
-MY_FSTAR=$(FSTAR) --cache_checked_modules $(FSTAR_OPTIONS)
-
-
-# a.fst(i).checked is the binary, checked version of a.fst(i)
-$(OUTPUT_DIRECTORY)/%.checked:
-	$(MY_FSTAR) $<
-
-all: extract
+all: verify
 
 parsers: verify
 	$(MAKE) -C parsers
 
 clean:
 	rm -rf *.checked .depend
-
-.depend: $(FSTAR_FILES)
-	$(MY_FSTAR) --dep full --extract 'Veritas -Veritas.SparseMerkleVerifier.Correctness' $^ > .depend
-
-depend: .depend
-
-include .depend
 
 verify: $(addprefix $(OUTPUT_DIRECTORY)/,$(addsuffix .checked, $(FSTAR_FILES)))
 driver: $(OUTPUT_DIRECTORY)/VeritasDriver.ml parsers VeritasDriver.fst
